theories/Examples/Examples01.v
@@ -1,0 +1,107 @@
+From Coq Require Import Lists.List.
+                 Import ListNotations.
+From Coq Require Import Strings.String.
+From Coq Require Import ZArith.
+
+From CoqUplc Require Import PlutusV3.Builtins.
+                     Import ExpectedArgNotations.
+From CoqUplc Require Import PlutusV3.CekMachine.
+From CoqUplc Require Import PlutusV3.CekValue.
+From CoqUplc Require Import PlutusV3.Uplc.
+
+Local Open Scope expectedArgs_scope.
+
+Definition integer_subtraction : program := 
+  (Program (Version 1 1 0)
+    (Apply (Apply (Builtin SubtractInteger) (Const (Integer 55%Z))) (Const (Integer 11%Z)))
+  ).
+
+Theorem example1_correctly_interpreted : cekExecuteProgram integer_subtraction nil 10 = Some (Halt (VCon (Integer 44))).
+Proof.
+  compute.
+  reflexivity.
+Qed.
+
+Definition integer_abs : program :=
+  (Program (Version 1 1 0)
+    (Lam "n"
+      (Apply
+        (Apply
+          (Apply
+            (Force (Builtin IfThenElse))
+              (Apply (Apply (Builtin LessThanInteger) (Var "n")) (Const (Integer 0)))
+          )
+          (Apply (Apply (Builtin SubtractInteger) (Const (Integer 0))) (Var "n"))
+        )
+        (Var "n")
+      )
+    )
+  ).
+
+Theorem example2_correctly_interpreted : cekExecuteProgram integer_abs [Const (Integer 5)] 37 = Some (Halt (VCon (Integer 5))).
+Proof.
+  compute.
+  reflexivity.
+Qed.
+
+Theorem example2_correct : forall (i : Z), cekExecuteProgram integer_abs [Const (Integer i)] 37 = Some (Halt (VCon (Integer (Z.abs i)))).
+Proof.
+  intros i.
+  induction i; compute; reflexivity.
+Qed.
+
+Definition integer_abs_lazy : program :=
+  (Program (Version 1 1 0)
+    (Lam "n"
+      (Apply
+        (Apply
+          (Apply
+            (Apply
+              (Force (Builtin IfThenElse))
+                (Apply (Apply (Builtin LessThanInteger) (Var "n")) (Const (Integer 0)))
+            )
+            (Lam "unit" (Apply (Apply (Builtin SubtractInteger) (Const (Integer 0))) (Var "n")))
+          )
+          (Lam "unit" (Var "n"))
+        )
+        (Const (Unit))
+      )
+    )
+  ).
+
+Theorem example3_correctly_interpreted : cekExecuteProgram integer_abs_lazy [Const (Integer 5)] 34 = Some (Halt (VCon (Integer 5))).
+Proof. 
+  compute.
+  reflexivity.
+Qed.
+
+Theorem example3_correct : forall (i : Z), cekExecuteProgram integer_abs_lazy [Const (Integer i)] 42 = Some (Halt (VCon (Integer (Z.abs i)))).
+Proof.
+  intros i.
+  induction i; compute; reflexivity.
+Qed.
+
+Definition integer_abs_lazy_delays : program :=
+  (Program (Version 1 1 0)
+    (Lam "n"
+      (Force
+        (Apply
+          (Apply
+            (Apply
+              (Force (Builtin IfThenElse))
+                (Apply (Apply (Builtin LessThanInteger) (Var "n")) (Const (Integer 0)))
+            )
+            (Delay (Apply (Apply (Builtin SubtractInteger) (Const (Integer 0))) (Var "n")))
+          )
+          (Delay (Var "n"))
+        )
+      )
+    )
+  ).
+
+Theorem example3_4_equivalence : forall (i : Z), cekExecuteProgram integer_abs_lazy_delays [Const (Integer i)] 42 =
+                                                 cekExecuteProgram integer_abs_lazy        [Const (Integer i)] 42.
+Proof.
+  intros i.
+  induction i; compute; reflexivity.
+Qed.
