theories/PlutusV3/BuiltinFunctions/Bool.v
@@ -1,0 +1,11 @@
+From Coq Require Import Lists.List.
+                 Import ListNotations.
+
+From CoqUplc Require Import PlutusV3.CekValue.
+From CoqUplc Require Import PlutusV3.Uplc.
+
+Definition ifThenElse (Vs : list cekValue) : option cekValue :=
+   match Vs with
+   | [VCon (Bool b); case_true; case_false] => Some (if b then case_true else case_false)
+   | _                                      => None
+   end.
