theories/PlutusV3/BuiltinFunctions/Evaluate.v
@@ -1,0 +1,13 @@
+From CoqUplc Require Import PlutusV3.CekValue.
+From CoqUplc Require Import PlutusV3.Uplc.
+
+From CoqUplc Require Import PlutusV3.BuiltinFunctions.Bool.
+From CoqUplc Require Import PlutusV3.BuiltinFunctions.Integer.
+
+Definition evaluate_builtin_function (b : builtinFun) : list cekValue -> option cekValue :=
+  match b with
+  | SubtractInteger => subtractInteger
+  | LessThanInteger => lessThanInteger
+  | IfThenElse      => ifThenElse
+  | _               => fun _ => None
+  end.
