theories/PlutusV3/BuiltinFunctions/Integer.v
@@ -1,0 +1,20 @@
+From Coq Require Import Lists.List.
+                 Import ListNotations.
+From Coq Require Import ZArith.
+
+From CoqUplc Require Import PlutusV3.CekValue.
+From CoqUplc Require Import PlutusV3.Uplc.
+
+Local Open Scope Z_scope.
+
+Definition subtractInteger (Vs : list cekValue) : option cekValue :=
+   match Vs with
+   | [VCon (Integer x); VCon (Integer y)] => Some (VCon (Integer (x - y)))
+   | _                                    => None
+   end.
+
+Definition lessThanInteger (Vs : list cekValue) : option cekValue :=
+  match Vs with
+   | [VCon (Integer x); VCon (Integer y)] => Some (VCon (Bool (x <=? y)))
+   | _                                    => None
+   end.
