theories/PlutusV3/CekValue.v
@@ -1,0 +1,15 @@
+From Coq Require Import Strings.String.
+
+From CoqUplc Require Import PlutusV3.Builtins.
+From CoqUplc Require Import PlutusV3.Uplc.
+
+Inductive cekValue : Set :=
+  | VCon     : const                                              -> cekValue
+  | VDelay   :           term -> environment                      -> cekValue
+  | VLam     : string -> term -> environment                      -> cekValue
+  | VConstr  : nat        -> list cekValue                        -> cekValue
+  | VBuiltin : builtinFun -> list cekValue -> expectedBuiltinArgs -> cekValue
+
+with environment : Set :=
+  | NonEmptyEnvironment : environment -> string -> cekValue -> environment
+  | EmptyEnvironment    :                                      environment.
